---
aliases: 
tags: 
origins: 
---
# Problem 3

### From $U_{1},U_{2}$ to $R,\Theta$
Consider that 
- $U_{1}=\frac{\Theta}{2\pi}$, $\frac{dU_{1}}{d\Theta}=\frac{1}{2\pi}$
- $U_{2}=\exp\left( -\frac{R^{2}}{2} \right)$, $\frac{dU_{2}}{dR}=R\exp\left( -\frac{R^{2}}{2} \right)$
Using change of variables  we have:
- $f_{\Theta}(\theta)=\frac{1}{2\pi}$
- $f_{R}(r)=r \exp\left( -\frac{r^{2}}{2} \right)$
### From $R,\Theta$ to $Z_{1},Z_{2}$
Note that: 
1. $Z_{1}^{2}+Z_{2}^{2}=R^{2}(\cos ^{2}\Theta+\sin ^{2}\Theta)=R^{2}$ thus $R=\sqrt{ Z_{1}^{2}+Z_{2}^{2} }$
    - $\frac{dR}{dZ_{1}}=Z_{1}(Z_{1}^{2}+Z_{2}^{2})^{-1/2}=\frac{Z_{1}}{R}$
    - Symmetrically $\frac{dR}{dZ_{2}}=\frac{Z_{2}}{R}$
2. $\frac{Z_{2}}{Z_{1}}=\frac{R\sin \Theta}{R\cos \Theta}=\tan \Theta$ thus $\Theta=\arctan\left( \frac{Z_{2}}{Z_{1}} \right)$
    - $\frac{d\Theta}{dZ_{1}}=\frac{1}{1+\frac{Z_{2}^{2}}{Z_{1}^{2}}}\cdot Z_{2}(-1)Z_{1}^{-2}=-\frac{Z_{2}}{Z_{1}^{2}+Z_{2}^{2}}=-\frac{Z_{2}}{R^{2}}$
    - Symmetrically $\frac{d\Theta}{dZ_{2}}=\frac{Z_{1}}{Z_{1}^{2}+Z_{2}^{2}}=\frac{Z_{1}}{R^{2}}$
Now, calculate the jacobian for a multivariate change of variables:

$$
\begin{align}
|J|&=\begin{vmatrix}
\frac{ \partial r  }{ \partial z_{1} }  & \frac{ \partial r }{ \partial z_{2} } \\
\frac{ \partial \theta }{ \partial z_{1} } & \frac{ \partial \theta }{ \partial z_{2} }    
\end{vmatrix} \\
&=\begin{vmatrix}
\frac{Z_{1}}{R} & \frac{Z_{2}}{R} \\
-\frac{Z_{2}}{R^{2}}  & \frac{Z_{1}}{R^{2}}
\end{vmatrix} \\
&= \frac{Z_{1}^{2}}{R^{3}}+ \frac{Z_{2}^{2}}{R^{3}} \\
&=\frac{1}{R}
\end{align}
$$
And thus the join probability being:
$$
\begin{align}
f_{\Theta,R}(\theta,r)&=f_{\Theta}(\theta)\cdot f_{R}(r)\cdot |J|\\
&=\frac{1}{2\pi}r\exp\left( -\frac{r^{2}}{2} \right)\cdot \frac{{1}}{r} \\
&= \frac{1}{2\pi}\exp\left(- \frac{z_{1}^{2}+z_{2}^{2}}{2} \right) \\
&=  \frac{1}{\sqrt{ 2\pi }}\exp\left( -\frac{z_{1}^{2}}{2} \right) \cdot  \frac{1}{\sqrt{ 2\pi }}\exp\left( -\frac{z_{2}^{2}}{2} \right) \\
&=f_{Z_{1}}(z_{1})\cdot f_{Z_{2}}(z_{2})
\end{align}
$$

This show both that:
1. $f_{Z_{1}},f_{Z_{2}}$ is the standard normal pdf
2. $Z_{1},Z_{2}$ are independent because the joint pdf is a simple product of each pdf. âˆŽ

