---
aliases: 
tags:
  - Courses
---


## Problem 1


## Problem 2

### Subproblem 1

Simply reporting $\infty$ utility on every item will result in the agent getting all items and thus maximum utility.

### Subproblem 2

Mechanism $A$ will calculate MNW $x^{*}= \text{argmax}_{x}\sum_{\forall i}\ln U_{i}(x)$ with the final allocation for agent $i$ being:
$$
x^{F}_{i}= x^{*}_{i} \frac{\prod_{j\neq i} U_{j}(x^{*})}{\prod_{j\neq i}U_{j}(x^{*}_{-i})}
$$
where, per the problem $x^{*}_{-i}= \text{argmax}_{x}\sum_{j\neq i}\ln U_{j}(x)$, i.e. running MNW without agent $i$. For agent $i$, their final utility is 
$$
U^{F}_{i}=U_{i}(x_{i}^{*} \frac{\prod_{j\neq i} U_{j}(x^{*})}{\prod_{j\neq i}U_{j}(x^{*}_{-i})})= U_{i}(x_{i}^{*})\cdot \frac{\prod_{j\neq i} U_{j}(x^{*})}{\prod_{j\neq i}U_{j}(x^{*}_{-i})}
$$
due to the utilities being additive utilities.
On the other hand, a VCG auction will allocate $x^{*}= \text{argmax}_{x}\sum_{\forall i}\ln b_{i}(x)$ where $b_{i}$ is the reported utility that may not be truthful. We consider agent $i$, while fixing everybody else's reported utilities $\vec{b_{-i}}$. The payment charged to agent $i$ is:
$$
\begin{align}
p_{i}&= \sum_{j\neq i}\ln b_{j}(x^{*}_{-i})- \underbrace{ \left( \sum_{\forall j}\ln b_{j}(x^{*})-\ln b_{i}(x^{*})U \right) }_{ =\sum_{j\neq i}\ln b_{j}(x^{*})  } & \text{per definition of VCG} \\
&= \ln \prod_{j\neq i}b_{j}(x_{-i}^{*})-\ln \prod_{j\neq i} b_{j}(x^{*}) \\
&= -\ln \left(\frac{\prod_{j\neq i} b_{j}(x^{*})}{\prod_{j\neq i}b_{j}(x^{*}_{-i})}\right)
\end{align}
$$
Thus for agent $i$ their final utility is
$$
\begin{align}
U_{i}^{F}& =\ln U_{i}(x^{*})- p_{i}  & \text{per the question}\\
& = \ln U_{i}(x^{*})+\ln \left(\frac{\prod_{j\neq i} b_{j}(x^{*})}{\prod_{j\neq i}b_{j}(x^{*}_{-i})}\right) \\
& = \ln\left(U_{i}(x^{*})\frac{\prod_{j\neq i} b_{j}(x^{*})}{\prod_{j\neq i}b_{j}(x^{*}_{-i})}\right)
\end{align}
$$
**Subproblem 2a**

Now, the correspondence comes from the fact that the subtraction of final utility due to VCG payment corresponds to the scaling down of utility in mechanism $A$. 

Specifically:
$$
\begin{align}
\ln f_{i}=\ln \prod_{j\neq i} U_{j}(x^{*}) -\ln\prod_{j\neq i}U_{j}(x^{*}_{-i}) \leq 0
\end{align}
$$
Since product of optimal utility allocation with $j$ divided by $U_{j}(x^{*})$, cannot be better than product of optimal utility allocation without $j$ in the first place (adaptation of logic from lecture). Thus we have $f_{i}\leq 1$.

**Subproblem 2b**
The correspondence between utilities will be:
$$
\ln U_{i}^{F,\text{Mech.A}} = U_{i}^{F,\text{VCG}}
$$
And since $\ln(x)$ is monotonic maximizing one will maximize the other. (Used in next proof)

**Subproblem 2c**

Considering the VCG mechanism, agent $i$ will attempt to maximize their own final utility, expressed as
$$
\begin{align}
U_{i}^{F,\text{VCG}}&=\ln U_{i}(x^{*})- \underbrace{ \ln \prod_{j\neq i}b_{j}(x_{-i}^{*}) }_\text{ i cannot influence }+\ln \prod_{j\neq i} b_{j}(x^{*}) \\
\text{max} U_{i}^{F,\text{Mech.A}} & \iff \text{max } U_{i}^{F,\text{VCG}} & \text{establised in 2b}\\
 & \iff \text{max} \left(\ln U_{i}(x^{*})+\ln \prod_{j\neq i}b_{j}(x^{*})\right) \\
& \iff  \text{max} \ln \prod_{\forall j}b_{j}(x^{*})  & \text{since $\vec{b_{-i}}$ is fixed}\\
& = \text{max} \sum _{\forall j} \ln b_{j}(x^{*}) & \text{Nash welfare max.}
\end{align}
$$
Which is to say, in mechanism $A$ it is also in $i$'s best interest to maximize the nash welfare objective. Thus mechanism $A$ is DSIC. <span style="float:right;">■</span>

**Subproblem 2d**

As outlined in the problem statement, for any allocation $\hat{x}$: 
$$
\begin{align}

\sum_{\forall i} \frac{U_{i}(\hat{x})}{U_{i}(x^{*})}  & \leq n & \text{remove specific agent $i$}\\
\sum_{j\neq i}^{n-1} \left(\frac{U_{j}(x^{*}_{-i})}{U_{j}(x^{*})}-1\right) & \leq 1 & \text{set } \hat{x}\coloneqq x_{-i}^{*}
\end{align}
$$
Now, using the hint from problem statement, set $d_{i}\coloneqq \frac{U_{j}(x_{-i}^{*})}{U_{j}(x^{*})}-1$ Then since $\sum_{j\neq i}^{n-1}d_{i}<1$, $\prod_{j\neq i}^{n-1}(d_{i}+1)\leq (1+\frac{1}{n-1})^{n-1}$. Then:
$$
\begin{align}
\left( \frac{n}{n-1} \right)^{n-1} &\geq \prod_{j\neq i}^{n-1}\frac{U_{j}(x^{*}_{-i})}{U_{j}(x^{*})} \\
& = \frac{\prod_{j\neq i} U_{j}(x^{*})}{\prod_{j\neq i}U_{j}(x^{*}_{-i})} \\
& = \frac{1}{f_{i}} \\
\lim_{ n \to \infty } \left( \frac{n}{n-1} \right)^{n-1} & \geq \lim_{ n \to \infty } \frac{1}{f_{i}} \\
\frac{1}{e} & \leq \lim_{ n \to \infty }  f_{i}
\end{align}
$$
<span style="float:right;">■</span>

## Problem 3

### Subproblem 1

Let allocation $A$ be EF1, i.e. $\forall i\forall j\exists g \text{ s.t. } v_{i}(A_{i})\geq v_{i}(A_{j}  \setminus \{ g \})$. Now, if we sum over all agents $j$ that is not $i$ on both sides:
$$
\begin{align}
\forall i\exists \vec{g} \text{ s.t. }(n-1)v_{i}(A_{i}) & \geq \sum_{j\neq i} v_{i}(A_{j} \setminus \{ g_{ij} \}) \\
nv_{i}(A_{i}) &\geq \sum_{j\neq i}v_{i}(A_{j} \setminus \{ g_{ij} \}) +v_{i}(A_{i}) & \text{adding $v_{i}(A_{i})$ to both sides} \\

& = \sum_{j\neq i}(v_{i}(A_{j})-v_{i}(\{ g_{ij} \}))+v_{i}(A_{i})\\

& =\sum_{j\neq i} v_{i}(A_{j})+v_{i}(A_{i})- \sum_{j\neq i}v_{i}(g_{ij}) \\
&= \sum_{\forall j}v_{i}\left( A_{j} \right) -\sum_{j\neq i}v_{i}(g_{ij})
\end{align}
$$
To bound each of these terms, we use:
$$
\begin{align}
\sum_{j\neq i}v_{i}(g_{ij}) & \leq \sum_{j\neq i} \text{max}_{g_{ij} \in A_{j}} v_{i}(g_{ij})  & \text{take item $i$ values most from everybody else}\\
& \leq (n-1) \text{max}_{g}v_{i}(g) & \text{just take maximum value item}
\end{align}
$$
Then returning to our original inequality:
$$
\begin{align}
nv_{i}(A_{i}) & \geq \underbrace{ \sum_{\forall j}v_{i}(A_{j}) }_{ =v_i(\bigcup_{\forall j}A_{j}) }- (n-1)\text{max}_{g}v_{i}(g) \\
\underbrace{ v_{i} (A_{i}) }_\text{ value of EF1 allocation to $i$ } & \geq \underbrace{ \frac{v_i(\bigcup_{\forall j}A_{j})}{n} }_\text{ value of proportional allocation to $i$ }-\underbrace{  \frac{n-1}{n}\text{max}_{g}v_{i}(g) }_\text{ some constant }
\end{align}
$$
<span style="float:right;">■</span>


## Problem 4

- let $X_{i}^{j}$ be the the utility of $i$ getting item $j$. Per the question this is $\text{Unif}[0,1]$.
- let $Y_{-i}^{j}$ be the largest utility an agent gives for item $j$, i.e. $Y_{-i}^{j}\coloneqq \text{max}_{k\neq i}X_{k}^{j}$.
- From this we know that the probability that agent $i$ will get item $j$ is $\mathbb{P}(X_{i}^{j}>Y_{-i}^{j})$
We first calculate $i$'s expected utility, $U_{i}$ from getting its own bundle:
$$
\begin{align}
\mathbb{E}(U_{i})\coloneqq &\mathbb{E}\left( \sum_{\forall j}X_{i}^{j} \underbrace{ \mathbb{1}_{X_{i}^{j}>Y_{-i}^{j}} }_\text{ i bid max? } \right)  \\
& = \sum_{\forall j}\underbrace{ \mathbb{E}(X_{i}^{j}\mid X_{i}^{j}>Y_{-i}^{j}) }_{=\frac{n}{n+1}\text{ , see explaination  below}}\underbrace{ \mathbb{P}(X_{i}^{j}>Y_{-i}^{j})  }_{=\frac{1}{n}  }\\
& =m\cdot \frac{n}{n+1} \cdot \frac{1}{n}
\end{align}
$$
Note that 
$$
\begin{align}
\mathbb{E}(X_{i}^{j}|X_{i}^{j}>Y_{-i}^{j}) & =\mathbb{E}(X_{i}^{j}\text{ given it is largest bid for }j) \\
 & =\mathbb{E}(n\text{-th smallest bid from $n$ i.i.d uniform r.v. 0 to 1}) \\
 & = \frac{n}{n+1}  & \text{Per the given hint}
\end{align}
$$
In a similar fashion, we can calculate $i$'s expected utility from getting another agent $k$'s bundle, $U_{ik}$:
$$
\begin{align}
\mathbb{E}(U_{ik})&\coloneqq \mathbb{E}\left( \sum_{\forall j} X_{i}^{j} \cdot \mathbb{1}_{X_{\textcolor{red}{ k }}^{j}>Y_{\textcolor{red}{ -k }}^{j}}\right)  \\
 & = \sum_{\forall j} \mathbb{E}(X_{i}^{j} | \underbrace{ X_{k}^{j}>Y_{-k}^{j} }_\text{ doesn't matter }) \cdot \mathbb{P}(X_{k}^{j}>Y_{-i}^{j}) \\
&= m \cdot \frac{1}{2} \cdot \frac{1}{n}
\end{align}
$$
Now, since the product $X_{i}^{j}\cdot \mathbb{1}_{X_{i}>Y_{-i}^{j}}$ themselves are independent random variables for all $i$, bounded from $[0,1]$, and considering that Hoeffding's inequality doesn't require identical distribution), we can use it to state:
$$
\begin{align}
\mathbb{P}(U_{i}\geq \mathbb{E}(U_{i})-t)  & \leq e^{ -2t^{2}/\sum_{\forall \text{items}}(1-0) } \\
 & = e^{ -2t^{2}/m }  \\
\mathbb{P}(U_{ik}\leq \mathbb{E}(U_{ik})+t) & \leq e^{ -2t^{2} /m}& \text{Equivalently}  
\end{align}
$$
Replacing $\mathbb{E}(U_{i}),\mathbb{E}(U_{ik})$ with the values we calculated above, as well as set $t\coloneqq \frac{m}{2(n+1)}$ we get:
$$
\begin{align}
\mathbb{P}\left( U_{i} \geq \frac{m}{2(n+1)} \right)\leq e^{ -m/2(n+1)^{2} } \\
\mathbb{P}\left( U_{ik} \leq \frac{3m}{2(n+1)} \right)\leq e^{ -m/2(n+1)^{2} }
\end{align}
$$
Now, the probability that $i$ will envy $k$ can be stated $\mathbb{P}(U_{i}<U_{ik})$. Using the union bound inequality:
$$
\begin{align}
\mathbb{P}(U_{i}<U_{ik})  & \leq \mathbb{P}\left( U_{i}\leq \frac{m}{2(n+1)} \text{and }U_{ik}\geq \frac{3m}{2(n+1)} \right) \\
& \leq \mathbb{P} \left( U_{i}\leq \frac{m}{2(n+1)} \right)+ \mathbb{P}\left( U_{ik}\leq \frac{3m}{2(n+1)} \right) \\
& \leq 2 e^{ -m/2(n+1)^{2} }
\end{align}
$$
Then, we calculate the probability that there will be no envy between any two agents $i,k$:
$$
\begin{align}
\mathbb{P}(\bigcup_{i,k}U_{i}<U_{ik})& \leq \underbrace{ \sum_{i} }_{n \text{ total agents, }  }\underbrace{ \sum_{k} }_{n \text{ total agents}  }\mathbb{P}(U_{i}<U_{ik}) \\
& = n^{2} 2e^{ -m/2(n+1)^{2} } \\
& \overset{ m \to \infty }{  \longrightarrow} 0
\end{align}

$$ 
<span style="float:right;">■</span>

